characterization_correctness.thy
@@ -1,0 +1,6 @@
+theory characterization_correctness
+  imports HML_list
+Transition_Systems
+begin
+
+end
